src/datalog/RelMap.v
@@ -9,6 +9,147 @@ From coqutil Require Import Map.Interface Map.Properties Map.Solver Tactics Tact
 
 Import ListNotations.
 
+Module normal_fact.
+  Section __.
+    Context `{params : datalog_params} {rel1 rel2 : Type}.
+
+    Definition map_rel (g : rel1 -> rel2) (nf : normal_fact (relt := rel1)) : normal_fact (relt := rel2) :=
+      {| normal_fact.rel := g nf.(normal_fact.rel);
+        normal_fact.args := nf.(normal_fact.args) |}.
+
+    Definition wf (wf_rel : rel1 -> rel2 -> Prop) (nf1 : normal_fact (relt := rel1)) (nf2 : normal_fact (relt := rel2)) :=
+      wf_rel nf1.(normal_fact.rel) nf2.(normal_fact.rel) /\
+        nf1.(normal_fact.args) = nf2.(normal_fact.args).
+  End __.
+End normal_fact.
+
+Module fact_pattern.
+  Section __.
+    Context `{params : datalog_params} {rel1 rel2 : Type}.
+
+    Definition map_rel (g : rel1 -> rel2) (fp : fact_pattern (relt := rel1)) : fact_pattern (relt := rel2) :=
+      {| fact_pattern.rel := g fp.(fact_pattern.rel);
+        fact_pattern.args := fp.(fact_pattern.args) |}.
+
+    Definition wf (wf_rel : rel1 -> rel2 -> Prop) (fp1 : fact_pattern (relt := rel1)) (fp2 : fact_pattern (relt := rel2)) :=
+      wf_rel fp1.(fact_pattern.rel) fp2.(fact_pattern.rel) /\
+        fp1.(fact_pattern.args) = fp2.(fact_pattern.args).
+  End __.
+End fact_pattern.
+
+Module meta_fact.
+  Section __.
+    Context `{params : datalog_params} {rel1 rel2 : Type}.
+
+    Definition map_rel (g : rel1 -> rel2) (mf : meta_fact (_rel := rel1)) : meta_fact (_rel := rel2) :=
+      {| meta_fact.pattern := fact_pattern.map_rel g mf.(meta_fact.pattern);
+        meta_fact.set := mf.(meta_fact.set);
+        meta_fact._pf := mf.(meta_fact._pf) |}.
+
+    Definition wf (wf_rel : rel1 -> rel2 -> Prop) (mf1 : meta_fact (_rel := rel1)) (mf2 : meta_fact (_rel := rel2)) :=
+      fact_pattern.wf wf_rel mf1.(meta_fact.pattern) mf2.(meta_fact.pattern) /\
+        mf1.(meta_fact.set) = mf2.(meta_fact.set).
+  End __.
+End meta_fact.
+
+Module fact.
+  Section __.
+    Context `{params : datalog_params} {rel1 rel2 : Type}.
+
+    Definition map_rel (g : rel1 -> rel2) (f : fact (_rel := rel1)) : fact (_rel := rel2) :=
+      match f with
+      | fact.normal nf => fact.normal (normal_fact.map_rel g nf)
+      | fact.meta mf => fact.meta (meta_fact.map_rel g mf)
+      end.
+
+    Definition wf (wf_rel : rel1 -> rel2 -> Prop) (f1 : fact (_rel := rel1)) (f2 : fact (_rel := rel2)) :=
+      match f1, f2 with
+      | fact.normal nf1, fact.normal nf2 => normal_fact.wf wf_rel nf1 nf2
+      | fact.meta mf1, fact.meta mf2 => meta_fact.wf wf_rel mf1 mf2
+      | _, _ => False
+      end.
+  End __.
+End fact.
+
+Module clause.
+  Section __.
+    Context `{params : datalog_params} {rel1 rel2 : Type}.
+
+    Definition map_rel (g : rel1 -> rel2) (c : clause (relt := rel1)) : clause (relt := rel2) :=
+      {| clause.rel := g c.(clause.rel);
+        clause.args := c.(clause.args) |}.
+
+    Definition wf (wf_rel : rel1 -> rel2 -> Prop) (c1 : clause (relt := rel1)) (c2 : clause (relt := rel2)) :=
+      wf_rel c1.(clause.rel) c2.(clause.rel) /\ c1.(clause.args) = c2.(clause.args).
+  End __.
+End clause.
+
+Module rule.
+  Section __.
+    Context `{params : datalog_params} {rel1 rel2 : Type}.
+
+    Definition map_rel (g : rel1 -> rel2) (r : rule (_rel := rel1)) : rule (_rel := rel2) :=
+      match r with
+      | rule.impl concls hyps =>
+          rule.impl (map (clause.map_rel g) concls) (map (clause.map_rel g) hyps)
+      | rule.agg concl agg hyp =>
+          rule.agg (g concl) agg (g hyp)
+      end.
+
+    Variant wf (wf_rel : rel1 -> rel2 -> Prop) : rule (_rel := rel1) -> rule (_rel := rel2) -> Prop :=
+      | wf_impl concls1 hyps1 concls2 hyps2 :
+        Forall2 (clause.wf wf_rel) concls1 concls2 ->
+        Forall2 (clause.wf wf_rel) hyps1 hyps2 ->
+        wf _ (rule.impl concls1 hyps1) (rule.impl concls2 hyps2)
+      | wf_agg concl1 concl2 a hyp1 hyp2 :
+        wf_rel concl1 concl2 ->
+        wf_rel hyp1 hyp2 ->
+        wf _ (rule.agg concl1 a hyp1) (rule.agg concl2 a hyp2).
+  End __.
+End rule.
+
+Module clause_pattern.
+  Section __.
+    Context `{params : datalog_params} {rel1 rel2 : Type}.
+
+    Definition map_rel (g : rel1 -> rel2) (cp : clause_pattern (relt := rel1)) : clause_pattern (relt := rel2) :=
+      {| clause_pattern.rel := g cp.(clause_pattern.rel);
+        clause_pattern.args := cp.(clause_pattern.args) |}.
+
+    Definition wf (wf_rel : rel1 -> rel2 -> Prop) (cp1 : clause_pattern (relt := rel1)) (cp2 : clause_pattern (relt := rel2)) :=
+      wf_rel cp1.(clause_pattern.rel) cp2.(clause_pattern.rel) /\
+        cp1.(clause_pattern.args) = cp2.(clause_pattern.args).
+  End __.
+End clause_pattern.
+
+Module meta_rule.
+  Section __.
+    Context `{params : datalog_params} {rel1 rel2 : Type}.
+
+    Definition map_rel (g : rel1 -> rel2) (mr : meta_rule (relt := rel1)) : meta_rule (relt := rel2) :=
+      {| meta_rule.concls := map (clause_pattern.map_rel g) mr.(meta_rule.concls);
+        meta_rule.hyps := map (clause_pattern.map_rel g) mr.(meta_rule.hyps) |}.
+
+    Definition wf (wf_rel : rel1 -> rel2 -> Prop) (mr1 : meta_rule (relt := rel1)) (mr2 : meta_rule (relt := rel2)) :=
+      Forall2 (clause_pattern.wf wf_rel) mr1.(meta_rule.concls) mr2.(meta_rule.concls) /\
+        Forall2 (clause_pattern.wf wf_rel) mr1.(meta_rule.hyps) mr2.(meta_rule.hyps).
+  End __.
+End meta_rule.
+
+Module program.
+  Section __.
+    Context `{params : datalog_params} {rel1 rel2 : Type}.
+
+    Definition map_rel (g : rel1 -> rel2) (p : program (relt := rel1)) : program (relt := rel2) :=
+      {| program.rules := map (rule.map_rel g) p.(program.rules);
+        program.meta_rules := map (meta_rule.map_rel g) p.(program.meta_rules) |}.
+
+    Definition wf (wf_rel : rel1 -> rel2 -> Prop) (p1 : program (relt := rel1)) (p2 : program (relt := rel2)) :=
+      Forall2 (rule.wf wf_rel) p1.(program.rules) p2.(program.rules) /\
+        Forall2 (meta_rule.wf wf_rel) p1.(program.meta_rules) p2.(program.meta_rules).
+  End __.
+End program.
+
 Section RelMap.
   Context {exprvar : exprvarT} {fn : fnT} {aggregator : aggregatorT} {T : valueT}.
   Context {semantics : datalog_semantics fn aggregator T}.
@@ -55,113 +196,94 @@ Section RelMap.
     Proof. auto. Qed.
     Hint Resolve inj_on_elt_at inj_on_at : core.
 
-    Definition wf_normal_fact (nf1 : normal_fact (relt := rel1)) (nf2 : normal_fact (relt := rel2)) :=
-      wf_rel nf1.(normal_fact.rel) nf2.(normal_fact.rel) /\
-        nf1.(normal_fact.args) = nf2.(normal_fact.args).
-
-    Definition wf_fact_pattern (fp1 : fact_pattern (relt := rel1)) (fp2 : fact_pattern (relt := rel2)) :=
-      wf_rel fp1.(fact_pattern.rel) fp2.(fact_pattern.rel) /\
-        fp1.(fact_pattern.args) = fp2.(fact_pattern.args).
-
-    Definition wf_meta_fact (mf1 : meta_fact (_rel := rel1)) (mf2 : meta_fact (_rel := rel2)) :=
-      wf_fact_pattern mf1.(meta_fact.pattern) mf2.(meta_fact.pattern) /\
-        mf1.(meta_fact.set) = mf2.(meta_fact.set).
-
-    Definition wf_fact (f1 : fact (_rel := rel1)) (f2 : fact (_rel := rel2)) :=
-      match f1, f2 with
-      | fact.normal nf1, fact.normal nf2 => wf_normal_fact nf1 nf2
-      | fact.meta mf1, fact.meta mf2 => wf_meta_fact mf1 mf2
-      | _, _ => False
-      end.
-
     Lemma wf_fact_map_rel_r g h :
-      wf_fact h (fact.map_rel g h) <-> wf_rel (fact.rel h) (g (fact.rel h)).
+      fact.wf wf_rel h (fact.map_rel g h) <-> wf_rel (fact.rel h) (g (fact.rel h)).
     Proof.
-      destruct h; cbv [wf_fact wf_normal_fact wf_meta_fact wf_fact_pattern fact.rel meta_fact.rel
+      destruct h; cbv [fact.wf normal_fact.wf meta_fact.wf fact_pattern.wf fact.rel meta_fact.rel
                        fact.map_rel normal_fact.map_rel meta_fact.map_rel fact_pattern.map_rel];
         simpl; intuition.
     Qed.
 
     Lemma wf_fact_map_rel_l g h :
-      wf_fact (fact.map_rel g h) h <-> wf_rel (g (fact.rel h)) (fact.rel h).
+      fact.wf wf_rel (fact.map_rel g h) h <-> wf_rel (g (fact.rel h)) (fact.rel h).
     Proof.
-      destruct h; cbv [wf_fact wf_normal_fact wf_meta_fact wf_fact_pattern fact.rel meta_fact.rel
+      destruct h; cbv [fact.wf normal_fact.wf meta_fact.wf fact_pattern.wf fact.rel meta_fact.rel
                        fact.map_rel normal_fact.map_rel meta_fact.map_rel fact_pattern.map_rel];
         simpl; intuition.
     Qed.
 
     Lemma wf_fact_rel f1 f2 :
-      wf_fact f1 f2 ->
+      fact.wf wf_rel f1 f2 ->
       wf_rel (fact.rel f1) (fact.rel f2).
     Proof.
-      destruct f1, f2; cbv [wf_fact wf_normal_fact wf_meta_fact wf_fact_pattern meta_fact.rel];
+      destruct f1, f2; cbv [fact.wf normal_fact.wf meta_fact.wf fact_pattern.wf meta_fact.rel];
         simpl; intuition.
     Qed.
 
     Lemma wf_normal_fact_fun nf1 nf2 nf2' :
       functional_at nf1.(normal_fact.rel) ->
-      wf_normal_fact nf1 nf2 ->
-      wf_normal_fact nf1 nf2' ->
+      normal_fact.wf wf_rel nf1 nf2 ->
+      normal_fact.wf wf_rel nf1 nf2' ->
       nf2 = nf2'.
     Proof.
-      destruct nf2, nf2'. cbv [functional_at wf_normal_fact]. simpl. intros. fwd.
+      destruct nf2, nf2'. cbv [functional_at normal_fact.wf]. simpl. intros. fwd.
       f_equal; solve [eauto | congruence].
     Qed.
 
     Lemma wf_normal_fact_inj nf1 nf1' nf2 :
       inj_at nf1.(normal_fact.rel) nf1'.(normal_fact.rel) ->
-      wf_normal_fact nf1 nf2 ->
-      wf_normal_fact nf1' nf2 ->
+      normal_fact.wf wf_rel nf1 nf2 ->
+      normal_fact.wf wf_rel nf1' nf2 ->
       nf1 = nf1'.
     Proof.
-      destruct nf1, nf1'. cbv [inj_at wf_normal_fact]. simpl. intros. fwd.
+      destruct nf1, nf1'. cbv [inj_at normal_fact.wf]. simpl. intros. fwd.
       f_equal; solve [eauto | congruence].
     Qed.
 
     Lemma wf_fact_pattern_fun fp1 fp2 fp2' :
       functional_at fp1.(fact_pattern.rel) ->
-      wf_fact_pattern fp1 fp2 ->
-      wf_fact_pattern fp1 fp2' ->
+      fact_pattern.wf wf_rel fp1 fp2 ->
+      fact_pattern.wf wf_rel fp1 fp2' ->
       fp2 = fp2'.
     Proof.
-      destruct fp2, fp2'. cbv [functional_at wf_fact_pattern]. simpl. intros. fwd.
+      destruct fp2, fp2'. cbv [functional_at fact_pattern.wf]. simpl. intros. fwd.
       f_equal; solve [eauto | congruence].
     Qed.
 
     Lemma wf_fact_pattern_inj fp1 fp1' fp2 :
       inj_at fp1.(fact_pattern.rel) fp1'.(fact_pattern.rel) ->
-      wf_fact_pattern fp1 fp2 ->
-      wf_fact_pattern fp1' fp2 ->
+      fact_pattern.wf wf_rel fp1 fp2 ->
+      fact_pattern.wf wf_rel fp1' fp2 ->
       fp1 = fp1'.
     Proof.
-      destruct fp1, fp1'. cbv [inj_at wf_fact_pattern]. simpl. intros. fwd.
+      destruct fp1, fp1'. cbv [inj_at fact_pattern.wf]. simpl. intros. fwd.
       f_equal; solve [eauto | congruence].
     Qed.
 
     Lemma wf_meta_fact_fun mf1 mf2 mf2' :
       functional_at (meta_fact.rel mf1) ->
-      wf_meta_fact mf1 mf2 ->
-      wf_meta_fact mf1 mf2' ->
+      meta_fact.wf wf_rel mf1 mf2 ->
+      meta_fact.wf wf_rel mf1 mf2' ->
       mf2 = mf2'.
     Proof.
-      cbv [wf_meta_fact]. intros. fwd. apply meta_fact.eq_ext; [|congruence].
+      cbv [meta_fact.wf]. intros. fwd. apply meta_fact.eq_ext; [|congruence].
       eapply wf_fact_pattern_fun; eassumption.
     Qed.
 
     Lemma wf_meta_fact_inj mf1 mf1' mf2 :
       inj_at (meta_fact.rel mf1) (meta_fact.rel mf1') ->
-      wf_meta_fact mf1 mf2 ->
-      wf_meta_fact mf1' mf2 ->
+      meta_fact.wf wf_rel mf1 mf2 ->
+      meta_fact.wf wf_rel mf1' mf2 ->
       mf1 = mf1'.
     Proof.
-      cbv [wf_meta_fact]. intros. fwd. apply meta_fact.eq_ext; [|congruence].
+      cbv [meta_fact.wf]. intros. fwd. apply meta_fact.eq_ext; [|congruence].
       eapply wf_fact_pattern_inj; eassumption.
     Qed.
 
     Lemma wf_fact_fun f1 f2 f2' :
       functional_at (fact.rel f1) ->
-      wf_fact f1 f2 ->
-      wf_fact f1 f2' ->
+      fact.wf wf_rel f1 f2 ->
+      fact.wf wf_rel f1 f2' ->
       f2 = f2'.
     Proof.
       destruct f1, f2, f2'; simpl; intros; try contradiction;
@@ -170,80 +292,55 @@ Section RelMap.
 
     Lemma wf_fact_inj f1 f1' f2 :
       inj_at (fact.rel f1) (fact.rel f1') ->
-      wf_fact f1 f2 ->
-      wf_fact f1' f2 ->
+      fact.wf wf_rel f1 f2 ->
+      fact.wf wf_rel f1' f2 ->
       f1 = f1'.
     Proof.
       destruct f1, f1', f2; simpl; intros; try contradiction;
         f_equal; eauto using wf_normal_fact_inj, wf_meta_fact_inj.
     Qed.
 
-    Definition wf_clause (c1 : clause (relt := rel1)) (c2 : clause (relt := rel2)) :=
-      wf_rel c1.(clause.rel) c2.(clause.rel) /\ c1.(clause.args) = c2.(clause.args).
-
-    Variant wf_rule : rule (_rel := rel1) -> rule (_rel := rel2) -> Prop :=
-      | wf_impl concls1 hyps1 concls2 hyps2 :
-        Forall2 wf_clause concls1 concls2 ->
-        Forall2 wf_clause hyps1 hyps2 ->
-        wf_rule (rule.impl concls1 hyps1) (rule.impl concls2 hyps2)
-      | wf_agg concl1 concl2 a hyp1 hyp2 :
-        wf_rel concl1 concl2 ->
-        wf_rel hyp1 hyp2 ->
-        wf_rule (rule.agg concl1 a hyp1) (rule.agg concl2 a hyp2).
-
-    Definition wf_clause_pattern (cp1 : clause_pattern (relt := rel1)) (cp2 : clause_pattern (relt := rel2)) :=
-      wf_rel cp1.(clause_pattern.rel) cp2.(clause_pattern.rel) /\
-        cp1.(clause_pattern.args) = cp2.(clause_pattern.args).
-
-    Definition wf_meta_rule (mr1 : meta_rule (relt := rel1)) (mr2 : meta_rule (relt := rel2)) :=
-      Forall2 wf_clause_pattern mr1.(meta_rule.concls) mr2.(meta_rule.concls) /\
-        Forall2 wf_clause_pattern mr1.(meta_rule.hyps) mr2.(meta_rule.hyps).
-
-    Definition wf_program (p1 : program (relt := rel1)) (p2 : program (relt := rel2)) :=
-      Forall2 wf_rule p1.(program.rules) p2.(program.rules) /\
-        Forall2 wf_meta_rule p1.(program.meta_rules) p2.(program.meta_rules).
-
     Lemma wf_clauses_rels cs1 cs2 :
-      Forall2 wf_clause cs1 cs2 ->
+      Forall2 (clause.wf wf_rel) cs1 cs2 ->
       Forall2 wf_rel (map clause.rel cs1) (map clause.rel cs2).
     Proof.
       intros. rewrite <- Forall2_map_l, <- Forall2_map_r.
-      eapply Forall2_impl; [eassumption|]. cbv [wf_clause]. intros. fwd. assumption.
+      eapply Forall2_impl; [eassumption|]. cbv [clause.wf]. intros. fwd. assumption.
     Qed.
 
     Lemma wf_clause_patterns_rels cs1 cs2 :
-      Forall2 wf_clause_pattern cs1 cs2 ->
+      Forall2 (clause_pattern.wf wf_rel) cs1 cs2 ->
       Forall2 wf_rel (map clause_pattern.rel cs1) (map clause_pattern.rel cs2).
     Proof.
       intros. rewrite <- Forall2_map_l, <- Forall2_map_r.
-      eapply Forall2_impl; [eassumption|]. cbv [wf_clause_pattern]. intros. fwd. assumption.
+      eapply Forall2_impl; [eassumption|]. cbv [clause_pattern.wf]. intros. fwd. assumption.
     Qed.
 
     Lemma wf_rule_hyp_rels r1 r2 :
-      wf_rule r1 r2 ->
+      rule.wf wf_rel r1 r2 ->
       Forall2 wf_rel (rule.hyp_rels r1) (rule.hyp_rels r2).
     Proof. destruct 1; simpl; eauto using wf_clauses_rels. Qed.
 
     Lemma wf_rule_concl_rels r1 r2 :
-      wf_rule r1 r2 ->
+      rule.wf wf_rel r1 r2 ->
       Forall2 wf_rel (rule.concl_rels r1) (rule.concl_rels r2).
     Proof. destruct 1; simpl; eauto using wf_clauses_rels. Qed.
 
     Lemma wf_meta_rule_hyp_rels mr1 mr2 :
-      wf_meta_rule mr1 mr2 ->
+      meta_rule.wf wf_rel mr1 mr2 ->
       Forall2 wf_rel (meta_rule.hyp_rels mr1) (meta_rule.hyp_rels mr2).
-    Proof. cbv [wf_meta_rule]. intros. fwd. eauto using wf_clause_patterns_rels. Qed.
+    Proof. cbv [meta_rule.wf]. intros. fwd. eauto using wf_clause_patterns_rels. Qed.
 
     Lemma wf_meta_rule_concl_rels mr1 mr2 :
-      wf_meta_rule mr1 mr2 ->
+      meta_rule.wf wf_rel mr1 mr2 ->
       Forall2 wf_rel (meta_rule.concl_rels mr1) (meta_rule.concl_rels mr2).
-    Proof. cbv [wf_meta_rule]. intros. fwd. eauto using wf_clause_patterns_rels. Qed.
+    Proof. cbv [meta_rule.wf]. intros. fwd. eauto using wf_clause_patterns_rels. Qed.
 
     Lemma wf_program_hyp_rels p1 p2 :
-      wf_program p1 p2 ->
+      program.wf wf_rel p1 p2 ->
       Forall2 wf_rel (program.hyp_rels p1) (program.hyp_rels p2).
     Proof.
-      cbv [wf_program program.hyp_rels]. intros. fwd. apply Forall2_app.
+      cbv [program.wf program.hyp_rels]. intros. fwd. apply Forall2_app.
       - apply Forall2_flat_map. eapply Forall2_impl; [eassumption|].
         eauto using wf_rule_hyp_rels.
       - apply Forall2_flat_map. eapply Forall2_impl; [eassumption|].
@@ -251,10 +348,10 @@ Section RelMap.
     Qed.
 
     Lemma wf_program_concl_rels p1 p2 :
-      wf_program p1 p2 ->
+      program.wf wf_rel p1 p2 ->
       Forall2 wf_rel (program.concl_rels p1) (program.concl_rels p2).
     Proof.
-      cbv [wf_program program.concl_rels]. intros. fwd. apply Forall2_app.
+      cbv [program.wf program.concl_rels]. intros. fwd. apply Forall2_app.
       - apply Forall2_flat_map. eapply Forall2_impl; [eassumption|].
         eauto using wf_rule_concl_rels.
       - apply Forall2_flat_map. eapply Forall2_impl; [eassumption|].
@@ -262,53 +359,53 @@ Section RelMap.
     Qed.
 
     Lemma clause_interp_wf ctx c1 c2 h1 :
-      wf_clause c1 c2 ->
+      clause.wf wf_rel c1 c2 ->
       clause.interp ctx c1 h1 ->
-      exists h2, wf_normal_fact h1 h2 /\ clause.interp ctx c2 h2.
+      exists h2, normal_fact.wf wf_rel h1 h2 /\ clause.interp ctx c2 h2.
     Proof.
-      cbv [wf_clause clause.interp wf_normal_fact]. intros. fwd.
+      cbv [clause.wf clause.interp normal_fact.wf]. intros. fwd.
       exists {| normal_fact.rel := c2.(clause.rel); normal_fact.args := h1.(normal_fact.args) |}.
       simpl. ssplit; congruence.
     Qed.
 
     Lemma clause_interp_wf_inv ctx c1 c2 h2 :
-      wf_clause c1 c2 ->
+      clause.wf wf_rel c1 c2 ->
       clause.interp ctx c2 h2 ->
-      exists h1, wf_normal_fact h1 h2 /\ clause.interp ctx c1 h1.
+      exists h1, normal_fact.wf wf_rel h1 h2 /\ clause.interp ctx c1 h1.
     Proof.
-      cbv [wf_clause clause.interp wf_normal_fact]. intros. fwd.
+      cbv [clause.wf clause.interp normal_fact.wf]. intros. fwd.
       exists {| normal_fact.rel := c1.(clause.rel); normal_fact.args := h2.(normal_fact.args) |}.
       simpl. ssplit; congruence.
     Qed.
 
     Lemma Forall2_clause_interp_wf ctx cs1 cs2 hs1 :
-      Forall2 wf_clause cs1 cs2 ->
+      Forall2 (clause.wf wf_rel) cs1 cs2 ->
       Forall2 (clause.interp ctx) cs1 hs1 ->
-      exists hs2, Forall2 wf_normal_fact hs1 hs2 /\ Forall2 (clause.interp ctx) cs2 hs2.
+      exists hs2, Forall2 (normal_fact.wf wf_rel) hs1 hs2 /\ Forall2 (clause.interp ctx) cs2 hs2.
     Proof.
       intros Hwf H.
-      eapply Forall2_Forall2_exists with (T := wf_normal_fact) (U := clause.interp ctx) in Hwf;
+      eapply Forall2_Forall2_exists with (T := normal_fact.wf wf_rel) (U := clause.interp ctx) in Hwf;
         [exact Hwf | exact H |].
       intros. eapply clause_interp_wf; eassumption.
     Qed.
 
     Lemma Forall2_clause_interp_wf_inv ctx cs1 cs2 hs2 :
-      Forall2 wf_clause cs1 cs2 ->
+      Forall2 (clause.wf wf_rel) cs1 cs2 ->
       Forall2 (clause.interp ctx) cs2 hs2 ->
-      exists hs1, Forall2 wf_normal_fact hs1 hs2 /\ Forall2 (clause.interp ctx) cs1 hs1.
+      exists hs1, Forall2 (normal_fact.wf wf_rel) hs1 hs2 /\ Forall2 (clause.interp ctx) cs1 hs1.
     Proof.
       intros Hwf H. rewrite <- Forall2_flip_iff in Hwf.
       eapply Forall2_Forall2_exists
-        with (T := fun h2 h1 => wf_normal_fact h1 h2) (U := clause.interp ctx) in Hwf;
+        with (T := fun h2 h1 => normal_fact.wf wf_rel h1 h2) (U := clause.interp ctx) in Hwf;
         [| exact H | intros; eapply clause_interp_wf_inv; eassumption].
       fwd. rewrite <- Forall2_flip_iff in Hwfp0. eauto.
     Qed.
 
     Lemma rule_interp_wf r1 r2 nf1 hyps1 :
-      wf_rule r1 r2 ->
+      rule.wf wf_rel r1 r2 ->
       rule.interp r1 nf1 hyps1 ->
       exists nf2 hyps2,
-        wf_normal_fact nf1 nf2 /\ Forall2 wf_fact hyps1 hyps2 /\ rule.interp r2 nf2 hyps2.
+        normal_fact.wf wf_rel nf1 nf2 /\ Forall2 (fact.wf wf_rel) hyps1 hyps2 /\ rule.interp r2 nf2 hyps2.
     Proof.
       intros Hwf Hint. destruct Hwf; invert Hint.
       - apply Exists_exists in H3. fwd.
@@ -331,19 +428,19 @@ Section RelMap.
                        fact.normal {| normal_fact.rel := hyp2;
                                      normal_fact.args := i :: x_i :: args |}) vals).
         ssplit.
-        + cbv [wf_normal_fact]. auto.
+        + cbv [normal_fact.wf]. auto.
         + constructor.
-          * cbv [wf_fact wf_meta_fact wf_fact_pattern meta_fact.mk]. auto.
+          * cbv [fact.wf meta_fact.wf fact_pattern.wf meta_fact.mk]. auto.
           * apply Forall2_map_map, Forall_forall. intros [i x] _.
-            cbv [wf_fact wf_normal_fact]. auto.
+            cbv [fact.wf normal_fact.wf]. auto.
         + constructor. assumption.
     Qed.
 
     Lemma rule_interp_wf_inv r1 r2 nf2 hyps2 :
-      wf_rule r1 r2 ->
+      rule.wf wf_rel r1 r2 ->
       rule.interp r2 nf2 hyps2 ->
       exists nf1 hyps1,
-        wf_normal_fact nf1 nf2 /\ Forall2 wf_fact hyps1 hyps2 /\ rule.interp r1 nf1 hyps1.
+        normal_fact.wf wf_rel nf1 nf2 /\ Forall2 (fact.wf wf_rel) hyps1 hyps2 /\ rule.interp r1 nf1 hyps1.
     Proof.
       intros Hwf Hint. destruct Hwf; invert Hint.
       - apply Exists_exists in H3. fwd.
@@ -366,70 +463,70 @@ Section RelMap.
                        fact.normal {| normal_fact.rel := hyp1;
                                      normal_fact.args := i :: x_i :: args |}) vals).
         ssplit.
-        + cbv [wf_normal_fact]. auto.
+        + cbv [normal_fact.wf]. auto.
         + constructor.
-          * cbv [wf_fact wf_meta_fact wf_fact_pattern meta_fact.mk]. auto.
+          * cbv [fact.wf meta_fact.wf fact_pattern.wf meta_fact.mk]. auto.
           * apply Forall2_map_map, Forall_forall. intros [i x] _.
-            cbv [wf_fact wf_normal_fact]. auto.
+            cbv [fact.wf normal_fact.wf]. auto.
         + constructor. assumption.
     Qed.
 
     Lemma clause_pattern_interp_wf ctx c1 c2 fp1 :
-      wf_clause_pattern c1 c2 ->
+      clause_pattern.wf wf_rel c1 c2 ->
       clause_pattern.interp ctx c1 fp1 ->
-      exists fp2, wf_fact_pattern fp1 fp2 /\ clause_pattern.interp ctx c2 fp2.
+      exists fp2, fact_pattern.wf wf_rel fp1 fp2 /\ clause_pattern.interp ctx c2 fp2.
     Proof.
-      cbv [wf_clause_pattern clause_pattern.interp wf_fact_pattern]. intros. fwd.
+      cbv [clause_pattern.wf clause_pattern.interp fact_pattern.wf]. intros. fwd.
       exists {| fact_pattern.rel := c2.(clause_pattern.rel);
                fact_pattern.args := fp1.(fact_pattern.args) |}.
       simpl. ssplit; congruence.
     Qed.
 
     Lemma clause_pattern_interp_wf_inv ctx c1 c2 fp2 :
-      wf_clause_pattern c1 c2 ->
+      clause_pattern.wf wf_rel c1 c2 ->
       clause_pattern.interp ctx c2 fp2 ->
-      exists fp1, wf_fact_pattern fp1 fp2 /\ clause_pattern.interp ctx c1 fp1.
+      exists fp1, fact_pattern.wf wf_rel fp1 fp2 /\ clause_pattern.interp ctx c1 fp1.
     Proof.
-      cbv [wf_clause_pattern clause_pattern.interp wf_fact_pattern]. intros. fwd.
+      cbv [clause_pattern.wf clause_pattern.interp fact_pattern.wf]. intros. fwd.
       exists {| fact_pattern.rel := c1.(clause_pattern.rel);
                fact_pattern.args := fp2.(fact_pattern.args) |}.
       simpl. ssplit; congruence.
     Qed.
 
     Lemma Forall2_clause_pattern_interp_wf ctx cs1 cs2 fps1 :
-      Forall2 wf_clause_pattern cs1 cs2 ->
+      Forall2 (clause_pattern.wf wf_rel) cs1 cs2 ->
       Forall2 (clause_pattern.interp ctx) cs1 fps1 ->
       exists fps2,
-        Forall2 wf_fact_pattern fps1 fps2 /\ Forall2 (clause_pattern.interp ctx) cs2 fps2.
+        Forall2 (fact_pattern.wf wf_rel) fps1 fps2 /\ Forall2 (clause_pattern.interp ctx) cs2 fps2.
     Proof.
       intros Hwf H.
       eapply Forall2_Forall2_exists
-        with (T := wf_fact_pattern) (U := clause_pattern.interp ctx) in Hwf;
+        with (T := fact_pattern.wf wf_rel) (U := clause_pattern.interp ctx) in Hwf;
         [exact Hwf | exact H |].
       intros. eapply clause_pattern_interp_wf; eassumption.
     Qed.
 
     Lemma Forall2_clause_pattern_interp_wf_inv ctx cs1 cs2 fps2 :
-      Forall2 wf_clause_pattern cs1 cs2 ->
+      Forall2 (clause_pattern.wf wf_rel) cs1 cs2 ->
       Forall2 (clause_pattern.interp ctx) cs2 fps2 ->
       exists fps1,
-        Forall2 wf_fact_pattern fps1 fps2 /\ Forall2 (clause_pattern.interp ctx) cs1 fps1.
+        Forall2 (fact_pattern.wf wf_rel) fps1 fps2 /\ Forall2 (clause_pattern.interp ctx) cs1 fps1.
     Proof.
       intros Hwf H. rewrite <- Forall2_flip_iff in Hwf.
       eapply Forall2_Forall2_exists
-        with (T := fun fp2 fp1 => wf_fact_pattern fp1 fp2) (U := clause_pattern.interp ctx) in Hwf;
+        with (T := fun fp2 fp1 => fact_pattern.wf wf_rel fp1 fp2) (U := clause_pattern.interp ctx) in Hwf;
         [| exact H | intros; eapply clause_pattern_interp_wf_inv; eassumption].
       fwd. rewrite <- Forall2_flip_iff in Hwfp0. eauto.
     Qed.
 
     Lemma pattern_interp_wf mr1 mr2 pat1 pats1 :
-      wf_meta_rule mr1 mr2 ->
+      meta_rule.wf wf_rel mr1 mr2 ->
       meta_rule.pattern_interp mr1 pat1 pats1 ->
       exists pat2 pats2,
-        wf_fact_pattern pat1 pat2 /\ Forall2 wf_fact_pattern pats1 pats2 /\
+        fact_pattern.wf wf_rel pat1 pat2 /\ Forall2 (fact_pattern.wf wf_rel) pats1 pats2 /\
           meta_rule.pattern_interp mr2 pat2 pats2.
     Proof.
-      cbv [wf_meta_rule meta_rule.pattern_interp]. intros Hwf H. fwd.
+      cbv [meta_rule.wf meta_rule.pattern_interp]. intros Hwf H. fwd.
       eapply Forall2_In_l in Hp0p0; [|eassumption]. fwd.
       eapply clause_pattern_interp_wf in Hp0p1; [|eassumption]. fwd.
       eapply Forall2_clause_pattern_interp_wf in Hp1; [|eassumption]. fwd.
@@ -438,13 +535,13 @@ Section RelMap.
     Qed.
 
     Lemma pattern_interp_wf_inv mr1 mr2 pat2 pats2 :
-      wf_meta_rule mr1 mr2 ->
+      meta_rule.wf wf_rel mr1 mr2 ->
       meta_rule.pattern_interp mr2 pat2 pats2 ->
       exists pat1 pats1,
-        wf_fact_pattern pat1 pat2 /\ Forall2 wf_fact_pattern pats1 pats2 /\
+        fact_pattern.wf wf_rel pat1 pat2 /\ Forall2 (fact_pattern.wf wf_rel) pats1 pats2 /\
           meta_rule.pattern_interp mr1 pat1 pats1.
     Proof.
-      cbv [wf_meta_rule meta_rule.pattern_interp]. intros Hwf H. fwd.
+      cbv [meta_rule.wf meta_rule.pattern_interp]. intros Hwf H. fwd.
       eapply Forall2_In_r in Hp0p0; [|eassumption]. fwd.
       eapply clause_pattern_interp_wf_inv in Hp0p1; [|eassumption]. fwd.
       eapply Forall2_clause_pattern_interp_wf_inv in Hp1; [|eassumption]. fwd.
@@ -453,27 +550,27 @@ Section RelMap.
     Qed.
 
     Lemma wf_meta_fact_of_pattern pat1 mf2 :
-      wf_fact_pattern pat1 mf2.(meta_fact.pattern) ->
-      exists mf1, pat1 = mf1.(meta_fact.pattern) /\ wf_meta_fact mf1 mf2.
+      fact_pattern.wf wf_rel pat1 mf2.(meta_fact.pattern) ->
+      exists mf1, pat1 = mf1.(meta_fact.pattern) /\ meta_fact.wf wf_rel mf1 mf2.
     Proof.
       intros H. exists (meta_fact.map_rel (fun _ => pat1.(fact_pattern.rel)) mf2).
-      cbv [wf_fact_pattern wf_meta_fact meta_fact.map_rel fact_pattern.map_rel] in *.
+      cbv [fact_pattern.wf meta_fact.wf meta_fact.map_rel fact_pattern.map_rel] in *.
       destruct pat1. simpl in *. fwd. auto.
     Qed.
 
     Lemma wf_meta_facts_of_patterns pats1 mhyps2 :
-      Forall2 wf_fact_pattern pats1 (map meta_fact.pattern mhyps2) ->
-      exists mhyps1, pats1 = map meta_fact.pattern mhyps1 /\ Forall2 wf_meta_fact mhyps1 mhyps2.
+      Forall2 (fact_pattern.wf wf_rel) pats1 (map meta_fact.pattern mhyps2) ->
+      exists mhyps1, pats1 = map meta_fact.pattern mhyps1 /\ Forall2 (meta_fact.wf wf_rel) mhyps1 mhyps2.
     Proof.
       intros H. rewrite <- Forall2_flip_iff, <- Forall2_map_l in H.
-      eapply Forall2_exists_r_map with (R' := fun mf2 mf1 => wf_meta_fact mf1 mf2) in H;
+      eapply Forall2_exists_r_map with (R' := fun mf2 mf1 => meta_fact.wf wf_rel mf1 mf2) in H;
         [|eauto using wf_meta_fact_of_pattern]. fwd.
       rewrite <- Forall2_flip_iff in Hp1. eauto.
     Qed.
 
     Lemma Forall2_wf_fact_meta mhyps1 hyps2 :
-      Forall2 wf_fact (map fact.meta mhyps1) hyps2 ->
-      exists mhyps2, hyps2 = map fact.meta mhyps2 /\ Forall2 wf_meta_fact mhyps1 mhyps2.
+      Forall2 (fact.wf wf_rel) (map fact.meta mhyps1) hyps2 ->
+      exists mhyps2, hyps2 = map fact.meta mhyps2 /\ Forall2 (meta_fact.wf wf_rel) mhyps1 mhyps2.
     Proof.
       intros H. rewrite <- Forall2_map_l in H. eapply Forall2_exists_r_map; [eassumption|].
       intros mf1 [nf2|mf2]; simpl; [contradiction|]. eauto.
@@ -481,22 +578,22 @@ Section RelMap.
 
     Lemma covered_by_wf h1 h2 fp1 fp2 :
       functional_at (fact.rel h1) ->
-      wf_fact h1 h2 ->
-      wf_fact_pattern fp1 fp2 ->
+      fact.wf wf_rel h1 h2 ->
+      fact_pattern.wf wf_rel fp1 fp2 ->
       fact.covered_by h1 fp1 ->
       fact.covered_by h2 fp2.
     Proof.
       destruct h1 as [nf1|mf1], h2 as [nf2|mf2]; simpl; intros Hfun Hh Hfp Hcov;
         try contradiction.
-      - cbv [wf_normal_fact wf_fact_pattern fact_pattern.matches functional_at] in *. fwd.
+      - cbv [normal_fact.wf fact_pattern.wf fact_pattern.matches functional_at] in *. fwd.
         split; [apply Hfun | ]; congruence.
       - subst. eapply wf_fact_pattern_fun; [exact Hfun | exact Hfp |]. apply Hh.
     Qed.
 
     Lemma covered_by_pats_wf h1 h2 pats1 pats2 :
       functional_at (fact.rel h1) ->
-      wf_fact h1 h2 ->
-      Forall2 wf_fact_pattern pats1 pats2 ->
+      fact.wf wf_rel h1 h2 ->
+      Forall2 (fact_pattern.wf wf_rel) pats1 pats2 ->
       fact.covered_by_pats pats1 h1 ->
       fact.covered_by_pats pats2 h2.
     Proof.
@@ -507,13 +604,13 @@ Section RelMap.
 
     Lemma implied_by_mf_wf h1 h2 mf1 mf2 :
       functional_at (fact.rel h1) ->
-      wf_fact h1 h2 ->
-      wf_meta_fact mf1 mf2 ->
+      fact.wf wf_rel h1 h2 ->
+      meta_fact.wf wf_rel mf1 mf2 ->
       fact.implied_by_mf h1 mf1 ->
       fact.implied_by_mf h2 mf2.
     Proof.
       destruct h1 as [nf1|m1], h2 as [nf2|m2]; simpl; intros Hfun Hh Hmf H; try contradiction.
-      - cbv [wf_normal_fact wf_meta_fact wf_fact_pattern meta_fact.matches fact_pattern.matches
+      - cbv [normal_fact.wf meta_fact.wf fact_pattern.wf meta_fact.matches fact_pattern.matches
                functional_at meta_fact.rel] in *. fwd.
         ssplit; [apply Hfun | |]; congruence.
       - subst. eapply wf_meta_fact_fun; eassumption.
@@ -521,8 +618,8 @@ Section RelMap.
 
     Lemma implied_by_mfs_wf h1 h2 mfs1 mfs2 :
       functional_at (fact.rel h1) ->
-      wf_fact h1 h2 ->
-      Forall2 wf_meta_fact mfs1 mfs2 ->
+      fact.wf wf_rel h1 h2 ->
+      Forall2 (meta_fact.wf wf_rel) mfs1 mfs2 ->
       fact.implied_by_mfs mfs1 h1 ->
       fact.implied_by_mfs mfs2 h2.
     Proof.
@@ -535,8 +632,8 @@ Section RelMap.
        image of mf1 agrees with whatever implied the image of the hypothesis. *)
     Lemma implied_by_mf_wf_bw h1 h2 mf1 mf2 mf2' :
       functional_at (fact.rel h1) ->
-      wf_fact h1 h2 ->
-      wf_meta_fact mf1 mf2' ->
+      fact.wf wf_rel h1 h2 ->
+      meta_fact.wf wf_rel mf1 mf2' ->
       meta_fact.agree mf2 mf2' ->
       fact.implied_by_mf h2 mf2 ->
       fact.covered_by h1 mf1.(meta_fact.pattern) ->
@@ -544,7 +641,7 @@ Section RelMap.
     Proof.
       destruct h1 as [nf1|m1], h2 as [nf2|m2]; simpl; intros Hfun Hh Hmf Hagree H Hcov;
         try contradiction.
-      - cbv [wf_normal_fact wf_meta_fact wf_fact_pattern meta_fact.matches fact_pattern.matches
+      - cbv [normal_fact.wf meta_fact.wf fact_pattern.wf meta_fact.matches fact_pattern.matches
                functional_at meta_fact.agree meta_fact.rel] in *. fwd.
         split; [auto|]. rewrite Hmfp1, Hhp1.
         rewrite <- (Hagree nf2); [assumption | auto | split; [apply Hfun|]; congruence].
@@ -555,8 +652,8 @@ Section RelMap.
 
     Lemma implied_by_mfs_wf_bw h1 h2 mfs1 mfs2 :
       functional_at (fact.rel h1) ->
-      wf_fact h1 h2 ->
-      Forall2 wf_meta_fact mfs1 mfs2 ->
+      fact.wf wf_rel h1 h2 ->
+      Forall2 (meta_fact.wf wf_rel) mfs1 mfs2 ->
       meta_facts_agree mfs2 ->
       fact.implied_by_mfs mfs2 h2 ->
       fact.covered_by_pats (map meta_fact.pattern mfs1) h1 ->
@@ -573,13 +670,13 @@ Section RelMap.
 
     Lemma implied_by_mf_wf_bw_inj h1 h2 mf1 mf2 :
       inj_at (fact.rel h1) (meta_fact.rel mf1) ->
-      wf_fact h1 h2 ->
-      wf_meta_fact mf1 mf2 ->
+      fact.wf wf_rel h1 h2 ->
+      meta_fact.wf wf_rel mf1 mf2 ->
       fact.implied_by_mf h2 mf2 ->
       fact.implied_by_mf h1 mf1.
     Proof.
       destruct h1 as [nf1|m1], h2 as [nf2|m2]; simpl; intros Hinj Hh Hmf H; try contradiction.
-      - cbv [wf_normal_fact wf_meta_fact wf_fact_pattern meta_fact.matches fact_pattern.matches
+      - cbv [normal_fact.wf meta_fact.wf fact_pattern.wf meta_fact.matches fact_pattern.matches
                inj_at meta_fact.rel] in *. fwd.
         ssplit; [symmetry; eapply Hinj; [eassumption | congruence] | congruence | congruence].
       - subst. eapply wf_meta_fact_inj; eassumption.
@@ -587,8 +684,8 @@ Section RelMap.
 
     Lemma implied_by_mfs_wf_bw_inj h1 h2 mfs1 mfs2 :
       Forall (fun mf => inj_at (fact.rel h1) (meta_fact.rel mf)) mfs1 ->
-      wf_fact h1 h2 ->
-      Forall2 wf_meta_fact mfs1 mfs2 ->
+      fact.wf wf_rel h1 h2 ->
+      Forall2 (meta_fact.wf wf_rel) mfs1 mfs2 ->
       fact.implied_by_mfs mfs2 h2 ->
       fact.implied_by_mfs mfs1 h1.
     Proof.
@@ -599,7 +696,7 @@ Section RelMap.
     Qed.
 
     Section Program.
-      Context (p1 : program (relt := rel1)) (p2 : program (relt := rel2)) (Hwf : wf_program p1 p2)
+      Context (p1 : program (relt := rel1)) (p2 : program (relt := rel2)) (Hwf : program.wf wf_rel p1 p2)
         (Hfun : Forall functional_at (program.all_rels p1)).
 
       Lemma functional_at_concl x :
@@ -636,7 +733,7 @@ Section RelMap.
 
       Lemma wf_fact_exists h1 :
         In (fact.rel h1) (program.hyp_rels p1) ->
-        exists h2, wf_fact h1 h2.
+        exists h2, fact.wf wf_rel h1 h2.
       Proof.
         intros H. eapply Forall2_In_l in H; [|apply wf_program_hyp_rels; exact Hwf]. fwd.
         exists (fact.map_rel (fun _ => y) h1). apply wf_fact_map_rel_r. assumption.
@@ -644,15 +741,15 @@ Section RelMap.
 
       Lemma wf_fact_exists_inv h2 :
         In (fact.rel h2) (program.hyp_rels p2) ->
-        exists h1, wf_fact h1 h2.
+        exists h1, fact.wf wf_rel h1 h2.
       Proof.
         intros H. eapply Forall2_In_r in H; [|apply wf_program_hyp_rels; exact Hwf]. fwd.
         exists (fact.map_rel (fun _ => x) h2). apply wf_fact_map_rel_l. assumption.
       Qed.
 
       Lemma one_step_derives_wf mhyps1 mhyps2 nf1 nf2 :
-        Forall2 wf_meta_fact mhyps1 mhyps2 ->
-        wf_normal_fact nf1 nf2 ->
+        Forall2 (meta_fact.wf wf_rel) mhyps1 mhyps2 ->
+        normal_fact.wf wf_rel nf1 nf2 ->
         rule.one_step_derives p1.(program.rules) mhyps1 nf1 ->
         rule.one_step_derives p2.(program.rules) mhyps2 nf2.
       Proof.
@@ -682,9 +779,9 @@ Section RelMap.
           In mr1 p1.(program.meta_rules) ->
           meta_rule.pattern_interp mr1 pat1 (map meta_fact.pattern mhyps1) ->
           fact_pattern.matches pat1 nf1 ->
-          Forall2 wf_meta_fact mhyps1 mhyps2 ->
+          Forall2 (meta_fact.wf wf_rel) mhyps1 mhyps2 ->
           meta_facts_agree mhyps2 ->
-          wf_normal_fact nf1 nf2 ->
+          normal_fact.wf wf_rel nf1 nf2 ->
           rule.one_step_derives p2.(program.rules) mhyps2 nf2 ->
           rule.one_step_derives p1.(program.rules) mhyps1 nf1.
         Proof.
@@ -703,9 +800,9 @@ Section RelMap.
 
         Lemma meta_rule_interp_wf mr1 mr2 mf1 mf2 mhyps1 mhyps2 :
           In mr1 p1.(program.meta_rules) ->
-          wf_meta_rule mr1 mr2 ->
-          wf_meta_fact mf1 mf2 ->
-          Forall2 wf_meta_fact mhyps1 mhyps2 ->
+          meta_rule.wf wf_rel mr1 mr2 ->
+          meta_fact.wf wf_rel mf1 mf2 ->
+          Forall2 (meta_fact.wf wf_rel) mhyps1 mhyps2 ->
           meta_facts_agree mhyps2 ->
           meta_rule.interp p1.(program.rules) mr1 mf1 mhyps1 ->
           meta_rule.interp p2.(program.rules) mr2 mf2 mhyps2.
@@ -724,24 +821,24 @@ Section RelMap.
           intros nf2 Hmatch2.
           pose proof (Hset {| normal_fact.rel := meta_fact.rel mf1;
                              normal_fact.args := nf2.(normal_fact.args) |}) as Hset1.
-          cbv [wf_meta_fact wf_fact_pattern fact_pattern.matches meta_fact.rel] in *. fwd.
+          cbv [meta_fact.wf fact_pattern.wf fact_pattern.matches meta_fact.rel] in *. fwd.
           simpl in Hset1. rewrite <- Hmfp1, Hset1 by (split; congruence).
           split.
-          - eapply one_step_derives_wf; [eassumption|]. cbv [wf_normal_fact]. simpl.
+          - eapply one_step_derives_wf; [eassumption|]. cbv [normal_fact.wf]. simpl.
             split; congruence.
           - eapply one_step_derives_wf_bw; [eassumption | eassumption | | eassumption | eassumption |].
             + cbv [fact_pattern.matches]. simpl. split; congruence.
-            + cbv [wf_normal_fact]. simpl. split; congruence.
+            + cbv [normal_fact.wf]. simpl. split; congruence.
         Qed.
 
         Lemma meta_rule_interp_wf_bw mr1 mr2 mf1 mf2 mhyps2 :
           In mr1 p1.(program.meta_rules) ->
-          wf_meta_rule mr1 mr2 ->
-          wf_meta_fact mf1 mf2 ->
+          meta_rule.wf wf_rel mr1 mr2 ->
+          meta_fact.wf wf_rel mf1 mf2 ->
           meta_facts_agree mhyps2 ->
           meta_rule.interp p2.(program.rules) mr2 mf2 mhyps2 ->
           exists mhyps1,
-            Forall2 wf_meta_fact mhyps1 mhyps2 /\
+            Forall2 (meta_fact.wf wf_rel) mhyps1 mhyps2 /\
               meta_rule.interp p1.(program.rules) mr1 mf1 mhyps1.
         Proof.
           intros Hmr Hwfmr Hmf Hagree [Hpat Hset].
@@ -754,19 +851,19 @@ Section RelMap.
           intros nf1 Hmatch1.
           pose proof (Hset {| normal_fact.rel := meta_fact.rel mf2;
                              normal_fact.args := nf1.(normal_fact.args) |}) as Hset2.
-          cbv [wf_meta_fact wf_fact_pattern fact_pattern.matches meta_fact.rel] in *. fwd.
+          cbv [meta_fact.wf fact_pattern.wf fact_pattern.matches meta_fact.rel] in *. fwd.
           simpl in Hset2. rewrite Hmfp1, Hset2 by (split; congruence).
           split.
           - eapply one_step_derives_wf_bw; [eassumption | eassumption | | eassumption | eassumption |].
             + cbv [fact_pattern.matches]. simpl. split; congruence.
-            + cbv [wf_normal_fact]. simpl. split; congruence.
-          - eapply one_step_derives_wf; [eassumption|]. cbv [wf_normal_fact]. simpl.
+            + cbv [normal_fact.wf]. simpl. split; congruence.
+          - eapply one_step_derives_wf; [eassumption|]. cbv [normal_fact.wf]. simpl.
             split; congruence.
         Qed.
 
         Lemma interp_step_wf f1 f2 hyps1 hyps2 :
-          wf_fact f1 f2 ->
-          Forall2 wf_fact hyps1 hyps2 ->
+          fact.wf wf_rel f1 f2 ->
+          Forall2 (fact.wf wf_rel) hyps1 hyps2 ->
           facts_agree hyps2 ->
           program.interp_step p1 f1 hyps1 ->
           program.interp_step p2 f2 hyps2.
@@ -791,10 +888,10 @@ Section RelMap.
         Qed.
 
         Lemma interp_step_wf_bw f1 f2 hyps2 :
-          wf_fact f1 f2 ->
+          fact.wf wf_rel f1 f2 ->
           facts_agree hyps2 ->
           program.interp_step p2 f2 hyps2 ->
-          exists hyps1, Forall2 wf_fact hyps1 hyps2 /\ program.interp_step p1 f1 hyps1.
+          exists hyps1, Forall2 (fact.wf wf_rel) hyps1 hyps2 /\ program.interp_step p1 f1 hyps1.
         Proof.
           intros Hf Hagree H. invert H.
           - destruct f1 as [nf1|]; [|contradiction].
@@ -817,11 +914,11 @@ Section RelMap.
 
         Context (Q1 Q2 : fact -> Prop)
           (Hgood : program.good_input_set p1 Q1)
-          (HQ : forall f1 f2, wf_fact f1 f2 -> Q1 f1 <-> Q2 f2).
+          (HQ : forall f1 f2, fact.wf wf_rel f1 f2 -> Q1 f1 <-> Q2 f2).
 
         Lemma interp_wf_transport f1 f1' f2 :
-          wf_fact f1 f2 ->
-          wf_fact f1' f2 ->
+          fact.wf wf_rel f1 f2 ->
+          fact.wf wf_rel f1' f2 ->
           program.interp p1 Q1 f1 ->
           program.interp p1 Q1 f1'.
         Proof.
@@ -831,7 +928,7 @@ Section RelMap.
         Qed.
 
         Lemma facts_agree_of_interp hyps2 :
-          (forall h2, In h2 hyps2 -> exists h1, wf_fact h1 h2 /\ program.interp p1 Q1 h1) ->
+          (forall h2, In h2 hyps2 -> exists h1, fact.wf wf_rel h1 h2 /\ program.interp p1 Q1 h1) ->
           facts_agree hyps2.
         Proof.
           intros H mf2 mf2' Hin Hin'.
@@ -841,25 +938,25 @@ Section RelMap.
           assert (Hi'' : program.interp p1 Q1
                            (fact.meta (meta_fact.map_rel (fun _ => meta_fact.rel mf1) mf1'))).
           { eapply interp_wf_transport with (f1 := fact.meta mf1'); [eassumption| |eassumption].
-            cbv [wf_fact wf_meta_fact wf_fact_pattern fact_pattern.matches meta_fact.map_rel
+            cbv [fact.wf meta_fact.wf fact_pattern.wf fact_pattern.matches meta_fact.map_rel
                    fact_pattern.map_rel meta_fact.rel] in *. simpl. fwd. ssplit; congruence. }
           pose proof (program.meta_facts_consistent p1 Q1 _ _ (proj1 Hgood)
                         ltac:(intros; eapply fact.set_doesnt_lie_agree; [apply Hgood | eassumption..])
                         Hvalid Hi1 Hi'') as Hagree.
           specialize (Hagree {| normal_fact.rel := meta_fact.rel mf1;
                                normal_fact.args := nf.(normal_fact.args) |}).
-          cbv [wf_fact wf_meta_fact wf_fact_pattern fact_pattern.matches meta_fact.map_rel
+          cbv [fact.wf meta_fact.wf fact_pattern.wf fact_pattern.matches meta_fact.map_rel
                  fact_pattern.map_rel meta_fact.rel] in *. simpl in *. fwd.
           rewrite <- Hwf1p1, <- Hwf1'p1. apply Hagree; split; congruence.
         Qed.
 
         Lemma interp_wf f1 :
           program.interp p1 Q1 f1 ->
-          forall f2, wf_fact f1 f2 -> program.interp p2 Q2 f2.
+          forall f2, fact.wf wf_rel f1 f2 -> program.interp p2 Q2 f2.
         Proof.
           induction 1; intros f2 Hf2.
           - apply pftree.leaf. apply (HQ _ _ Hf2). assumption.
-          - edestruct (Forall_exists_r_Forall2 wf_fact l) as [hyps2 Hhyps2].
+          - edestruct (Forall_exists_r_Forall2 (fact.wf wf_rel) l) as [hyps2 Hhyps2].
             { eapply Forall_impl; [eapply program.interp_step_hyp_relname_in; eassumption|].
               simpl. eauto using wf_fact_exists. }
             rewrite Forall_forall in H0, H1.
@@ -873,7 +970,7 @@ Section RelMap.
 
         Lemma interp_wf_bw f2 :
           program.interp p2 Q2 f2 ->
-          forall f1, wf_fact f1 f2 -> program.interp p1 Q1 f1.
+          forall f1, fact.wf wf_rel f1 f2 -> program.interp p1 Q1 f1.
         Proof.
           induction 1; intros f1 Hf1.
           - apply pftree.leaf. apply (HQ _ _ Hf1). assumption.
@@ -916,8 +1013,8 @@ Section RelMap.
         Lemma one_step_derives_wf_bw_inj mhyps1 mhyps2 nf1 nf2 :
           In nf1.(normal_fact.rel) l ->
           Forall (fun mf => In (meta_fact.rel mf) l) mhyps1 ->
-          Forall2 wf_meta_fact mhyps1 mhyps2 ->
-          wf_normal_fact nf1 nf2 ->
+          Forall2 (meta_fact.wf wf_rel) mhyps1 mhyps2 ->
+          normal_fact.wf wf_rel nf1 nf2 ->
           rule.one_step_derives p2.(program.rules) mhyps2 nf2 ->
           rule.one_step_derives p1.(program.rules) mhyps1 nf1.
         Proof.
@@ -937,9 +1034,9 @@ Section RelMap.
 
         Lemma meta_rule_interp_wf_inj mr1 mr2 mf1 mf2 mhyps1 mhyps2 :
           In mr1 p1.(program.meta_rules) ->
-          wf_meta_rule mr1 mr2 ->
-          wf_meta_fact mf1 mf2 ->
-          Forall2 wf_meta_fact mhyps1 mhyps2 ->
+          meta_rule.wf wf_rel mr1 mr2 ->
+          meta_fact.wf wf_rel mf1 mf2 ->
+          Forall2 (meta_fact.wf wf_rel) mhyps1 mhyps2 ->
           meta_rule.interp p1.(program.rules) mr1 mf1 mhyps1 ->
           meta_rule.interp p2.(program.rules) mr2 mf2 mhyps2.
         Proof.
@@ -960,25 +1057,25 @@ Section RelMap.
           pose proof (Hset {| normal_fact.rel := meta_fact.rel mf1;
                              normal_fact.args := nf2.(normal_fact.args) |}) as Hset1.
           pose proof (meta_rule.pattern_interp_concl_relname_in _ _ _ Hpat) as Hconcl.
-          cbv [wf_meta_fact wf_fact_pattern fact_pattern.matches meta_fact.rel] in *. fwd.
+          cbv [meta_fact.wf fact_pattern.wf fact_pattern.matches meta_fact.rel] in *. fwd.
           simpl in Hset1. rewrite <- Hmfp1, Hset1 by (split; congruence).
           split.
-          - eapply one_step_derives_wf; [eassumption|]. cbv [wf_normal_fact]. simpl.
+          - eapply one_step_derives_wf; [eassumption|]. cbv [normal_fact.wf]. simpl.
             split; congruence.
           - eapply one_step_derives_wf_bw_inj; [| |eassumption|].
             + simpl. eauto 6.
             + eapply Forall_impl; [eassumption|]. eauto 6.
-            + cbv [wf_normal_fact]. simpl. split; congruence.
+            + cbv [normal_fact.wf]. simpl. split; congruence.
         Qed.
 
         Lemma meta_rule_interp_wf_bw_inj mr1 mr2 mf1 mf2 mhyps2 :
           In mr1 p1.(program.meta_rules) ->
           In (meta_fact.rel mf1) l ->
-          wf_meta_rule mr1 mr2 ->
-          wf_meta_fact mf1 mf2 ->
+          meta_rule.wf wf_rel mr1 mr2 ->
+          meta_fact.wf wf_rel mf1 mf2 ->
           meta_rule.interp p2.(program.rules) mr2 mf2 mhyps2 ->
           exists mhyps1,
-            Forall2 wf_meta_fact mhyps1 mhyps2 /\
+            Forall2 (meta_fact.wf wf_rel) mhyps1 mhyps2 /\
               meta_rule.interp p1.(program.rules) mr1 mf1 mhyps1.
         Proof.
           intros Hmr Hmf1 Hwfmr Hmf [Hpat Hset].
@@ -993,20 +1090,20 @@ Section RelMap.
           intros nf1 Hmatch1.
           pose proof (Hset {| normal_fact.rel := meta_fact.rel mf2;
                              normal_fact.args := nf1.(normal_fact.args) |}) as Hset2.
-          cbv [wf_meta_fact wf_fact_pattern fact_pattern.matches meta_fact.rel] in *. fwd.
+          cbv [meta_fact.wf fact_pattern.wf fact_pattern.matches meta_fact.rel] in *. fwd.
           simpl in Hset2. rewrite Hmfp1, Hset2 by (split; congruence).
           split.
           - eapply one_step_derives_wf_bw_inj; [| |eassumption|].
             + simpl. congruence.
             + eapply Forall_impl; [eassumption|]. eauto 6.
-            + cbv [wf_normal_fact]. simpl. split; congruence.
-          - eapply one_step_derives_wf; [eassumption|]. cbv [wf_normal_fact]. simpl.
+            + cbv [normal_fact.wf]. simpl. split; congruence.
+          - eapply one_step_derives_wf; [eassumption|]. cbv [normal_fact.wf]. simpl.
             split; congruence.
         Qed.
 
         Lemma interp_step_wf_inj f1 f2 hyps1 hyps2 :
-          wf_fact f1 f2 ->
-          Forall2 wf_fact hyps1 hyps2 ->
+          fact.wf wf_rel f1 f2 ->
+          Forall2 (fact.wf wf_rel) hyps1 hyps2 ->
           program.interp_step p1 f1 hyps1 ->
           program.interp_step p2 f2 hyps2.
         Proof.
@@ -1031,9 +1128,9 @@ Section RelMap.
 
         Lemma interp_step_wf_bw_inj f1 f2 hyps2 :
           In (fact.rel f1) l ->
-          wf_fact f1 f2 ->
+          fact.wf wf_rel f1 f2 ->
           program.interp_step p2 f2 hyps2 ->
-          exists hyps1, Forall2 wf_fact hyps1 hyps2 /\ program.interp_step p1 f1 hyps1.
+          exists hyps1, Forall2 (fact.wf wf_rel) hyps1 hyps2 /\ program.interp_step p1 f1 hyps1.
         Proof.
           intros Hf1 Hf H. invert H.
           - destruct f1 as [nf1|]; [|contradiction].
@@ -1055,15 +1152,15 @@ Section RelMap.
         Qed.
 
         Context (Q1 Q2 : fact -> Prop)
-          (HQ : forall f1 f2, wf_fact f1 f2 -> Q1 f1 <-> Q2 f2).
+          (HQ : forall f1 f2, fact.wf wf_rel f1 f2 -> Q1 f1 <-> Q2 f2).
 
         Lemma interp_wf_inj f1 :
           program.interp p1 Q1 f1 ->
-          forall f2, wf_fact f1 f2 -> program.interp p2 Q2 f2.
+          forall f2, fact.wf wf_rel f1 f2 -> program.interp p2 Q2 f2.
         Proof.
           induction 1; intros f2 Hf2.
           - apply pftree.leaf. apply (HQ _ _ Hf2). assumption.
-          - edestruct (Forall_exists_r_Forall2 wf_fact l0) as [hyps2 Hhyps2].
+          - edestruct (Forall_exists_r_Forall2 (fact.wf wf_rel) l0) as [hyps2 Hhyps2].
             { eapply Forall_impl; [eapply program.interp_step_hyp_relname_in; eassumption|].
               simpl. eauto using wf_fact_exists. }
             rewrite Forall_forall in H1.
@@ -1074,7 +1171,7 @@ Section RelMap.
 
         Lemma interp_wf_bw_inj f2 :
           program.interp p2 Q2 f2 ->
-          forall f1, wf_fact f1 f2 -> In (fact.rel f1) l -> program.interp p1 Q1 f1.
+          forall f1, fact.wf wf_rel f1 f2 -> In (fact.rel f1) l -> program.interp p1 Q1 f1.
         Proof.
           induction 1; intros f1 Hf1 Hl1.
           - apply pftree.leaf. apply (HQ _ _ Hf1). assumption.
@@ -1090,13 +1187,13 @@ Section RelMap.
     End Program.
 
     Theorem interp_wf_iff p1 p2 Q1 Q2 f1 f2 :
-      wf_program p1 p2 ->
+      program.wf wf_rel p1 p2 ->
       Forall functional_at (program.all_rels p1) ->
       Forall inj_on_elt (program.concl_rels p1) ->
       program.meta_rules_valid p1 ->
       program.good_input_set p1 Q1 ->
-      (forall g1 g2, wf_fact g1 g2 -> Q1 g1 <-> Q2 g2) ->
-      wf_fact f1 f2 ->
+      (forall g1 g2, fact.wf wf_rel g1 g2 -> Q1 g1 <-> Q2 g2) ->
+      fact.wf wf_rel f1 f2 ->
       program.interp p1 Q1 f1 <-> program.interp p2 Q2 f2.
     Proof.
       intros. split; intros H'.
@@ -1105,11 +1202,11 @@ Section RelMap.
     Qed.
 
     Theorem interp_wf_iff_inj p1 p2 Q1 Q2 f1 f2 :
-      wf_program p1 p2 ->
+      program.wf wf_rel p1 p2 ->
       Forall functional_at (program.all_rels p1) ->
       inj_on (fact.rel f1 :: program.all_rels p1) ->
-      (forall g1 g2, wf_fact g1 g2 -> Q1 g1 <-> Q2 g2) ->
-      wf_fact f1 f2 ->
+      (forall g1 g2, fact.wf wf_rel g1 g2 -> Q1 g1 <-> Q2 g2) ->
+      fact.wf wf_rel f1 f2 ->
       program.interp p1 Q1 f1 <-> program.interp p2 Q2 f2.
     Proof.
       intros. split; intros H'.
@@ -1119,7 +1216,7 @@ Section RelMap.
     Qed.
 
     Lemma meta_rules_valid_wf p1 p2 :
-      wf_program p1 p2 ->
+      program.wf wf_rel p1 p2 ->
       Forall functional_at (program.hyp_rels p1) ->
       inj_on (program.concl_rels p1) ->
       program.meta_rules_valid p1 ->
@@ -1134,7 +1231,7 @@ Section RelMap.
       rewrite Forall_forall in Hfun.
       specialize (Hvalid _ _ ltac:(eauto) ltac:(eauto) _ _ _ _ Hpat1p2 Hint1p2).
       specialize' Hvalid.
-      { cbv [wf_fact_pattern wf_normal_fact fact_pattern.matches] in *. fwd.
+      { cbv [fact_pattern.wf normal_fact.wf fact_pattern.matches] in *. fwd.
         rewrite Hmatch2p0 in Hpat1p0p0.
         split; [|congruence]. eapply Hinj; [| |eassumption..].
         - eauto using meta_rule.pattern_interp_concl_relname_in.
@@ -1153,11 +1250,11 @@ Section RelMap.
     Definition fact_equiv f1 f2 := fact.map_rel f f1 = fact.map_rel f f2.
 
     Lemma wf_fact_map g1 g2 :
-      wf_fact map_rel g1 g2 <-> fact.map_rel f g1 = g2.
+      fact.wf map_rel g1 g2 <-> fact.map_rel f g1 = g2.
     Proof.
       split; intros H.
       - destruct g1 as [nf1|mf1], g2 as [[r2 a2]|[[r2 a2] s2 p2]];
-          cbv [wf_fact wf_normal_fact wf_meta_fact wf_fact_pattern map_rel] in H; fwd;
+          cbv [fact.wf normal_fact.wf meta_fact.wf fact_pattern.wf map_rel] in H; fwd;
           try contradiction;
           cbv [fact.map_rel normal_fact.map_rel meta_fact.map_rel fact_pattern.map_rel]; simpl in *.
         + congruence.
@@ -1165,55 +1262,42 @@ Section RelMap.
       - subst. apply wf_fact_map_rel_r. reflexivity.
     Qed.
 
-    Definition map_clause_rel (c : clause) : clause :=
-      {| clause.rel := f c.(clause.rel);
-        clause.args := c.(clause.args) |}.
-
-    Definition map_clause_pattern_rel (c : clause_pattern) : clause_pattern :=
-      {| clause_pattern.rel := f c.(clause_pattern.rel);
-        clause_pattern.args := c.(clause_pattern.args) |}.
-
-    Definition map_rule_rels (r : rule) : rule :=
-      match r with
-      | rule.impl concls hyps =>
-          rule.impl (map map_clause_rel concls) (map map_clause_rel hyps)
-      | rule.agg concl agg hyp =>
-          rule.agg (f concl) agg (f hyp)
-      end.
-
-    Definition map_meta_rule_rels (r : meta_rule) : meta_rule :=
-      {| meta_rule.concls := map map_clause_pattern_rel r.(meta_rule.concls);
-        meta_rule.hyps := map map_clause_pattern_rel r.(meta_rule.hyps) |}.
-
-    Definition map_program (p : program) : program :=
-      {| program.rules := map map_rule_rels p.(program.rules);
-        program.meta_rules := map map_meta_rule_rels p.(program.meta_rules) |}.
+    Lemma map_fact_inj a b :
+      (f (fact.rel a) = f (fact.rel b) -> fact.rel a = fact.rel b) ->
+      fact.map_rel f a = fact.map_rel f b ->
+      a = b.
+    Proof.
+      intros Hinj H. eapply (wf_fact_inj map_rel).
+      - cbv [inj_at map_rel]. intros. apply Hinj. congruence.
+      - apply wf_fact_map. exact H.
+      - apply wf_fact_map. reflexivity.
+    Qed.
 
     Lemma wf_clauses_map cs :
-      Forall2 (wf_clause map_rel) cs (map map_clause_rel cs).
+      Forall2 (clause.wf map_rel) cs (map (clause.map_rel f) cs).
     Proof.
-      rewrite <- Forall2_map_r. apply Forall2_same, Forall_forall. cbv [wf_clause map_rel]. auto.
+      rewrite <- Forall2_map_r. apply Forall2_same, Forall_forall. cbv [clause.wf map_rel]. auto.
     Qed.
 
     Lemma wf_clause_patterns_map cs :
-      Forall2 (wf_clause_pattern map_rel) cs (map map_clause_pattern_rel cs).
+      Forall2 (clause_pattern.wf map_rel) cs (map (clause_pattern.map_rel f) cs).
     Proof.
       rewrite <- Forall2_map_r. apply Forall2_same, Forall_forall.
-      cbv [wf_clause_pattern map_rel]. auto.
+      cbv [clause_pattern.wf map_rel]. auto.
     Qed.
 
     Lemma wf_rule_map r :
-      wf_rule map_rel r (map_rule_rels r).
+      rule.wf map_rel r (rule.map_rel f r).
     Proof. destruct r; constructor; cbv [map_rel]; auto using wf_clauses_map. Qed.
 
     Lemma wf_meta_rule_map mr :
-      wf_meta_rule map_rel mr (map_meta_rule_rels mr).
-    Proof. cbv [wf_meta_rule map_meta_rule_rels]. simpl. split; apply wf_clause_patterns_map. Qed.
+      meta_rule.wf map_rel mr (meta_rule.map_rel f mr).
+    Proof. cbv [meta_rule.wf meta_rule.map_rel]. simpl. split; apply wf_clause_patterns_map. Qed.
 
     Lemma wf_program_map p :
-      wf_program map_rel p (map_program p).
+      program.wf map_rel p (program.map_rel f p).
     Proof.
-      cbv [wf_program map_program]. simpl.
+      cbv [program.wf program.map_rel]. simpl.
       split; rewrite <- Forall2_map_r; apply Forall2_same, Forall_forall;
         auto using wf_rule_map, wf_meta_rule_map.
     Qed.
@@ -1228,41 +1312,41 @@ Section RelMap.
     Proof. cbv [injective_on inj_on inj_at map_rel]. intros. subst. auto. Qed.
 
     Lemma concl_rels_map_rule_rels r :
-      rule.concl_rels (map_rule_rels r) = map f (rule.concl_rels r).
+      rule.concl_rels (rule.map_rel f r) = map f (rule.concl_rels r).
     Proof. destruct r; simpl; [rewrite !map_map|]; reflexivity. Qed.
 
     Lemma hyp_rels_map_rule_rels r :
-      rule.hyp_rels (map_rule_rels r) = map f (rule.hyp_rels r).
+      rule.hyp_rels (rule.map_rel f r) = map f (rule.hyp_rels r).
     Proof. destruct r; simpl; [rewrite !map_map|]; reflexivity. Qed.
 
     Lemma concl_rels_map_meta_rule_rels mr :
-      meta_rule.concl_rels (map_meta_rule_rels mr) = map f (meta_rule.concl_rels mr).
-    Proof. cbv [meta_rule.concl_rels map_meta_rule_rels]. simpl. rewrite !map_map. reflexivity. Qed.
+      meta_rule.concl_rels (meta_rule.map_rel f mr) = map f (meta_rule.concl_rels mr).
+    Proof. cbv [meta_rule.concl_rels meta_rule.map_rel]. simpl. rewrite !map_map. reflexivity. Qed.
 
     Lemma hyp_rels_map_meta_rule_rels mr :
-      meta_rule.hyp_rels (map_meta_rule_rels mr) = map f (meta_rule.hyp_rels mr).
-    Proof. cbv [meta_rule.hyp_rels map_meta_rule_rels]. simpl. rewrite !map_map. reflexivity. Qed.
+      meta_rule.hyp_rels (meta_rule.map_rel f mr) = map f (meta_rule.hyp_rels mr).
+    Proof. cbv [meta_rule.hyp_rels meta_rule.map_rel]. simpl. rewrite !map_map. reflexivity. Qed.
 
     Lemma concl_rels_map_program p :
-      program.concl_rels (map_program p) = map f (program.concl_rels p).
+      program.concl_rels (program.map_rel f p) = map f (program.concl_rels p).
     Proof.
-      cbv [program.concl_rels map_program]. simpl.
+      cbv [program.concl_rels program.map_rel]. simpl.
       rewrite map_app, !map_flat_map, !flat_map_map. f_equal.
       - apply flat_map_ext. apply concl_rels_map_rule_rels.
       - apply flat_map_ext. apply concl_rels_map_meta_rule_rels.
     Qed.
 
     Lemma hyp_rels_map_program p :
-      program.hyp_rels (map_program p) = map f (program.hyp_rels p).
+      program.hyp_rels (program.map_rel f p) = map f (program.hyp_rels p).
     Proof.
-      cbv [program.hyp_rels map_program]. simpl.
+      cbv [program.hyp_rels program.map_rel]. simpl.
       rewrite map_app, !map_flat_map, !flat_map_map. f_equal.
       - apply flat_map_ext. apply hyp_rels_map_rule_rels.
       - apply flat_map_ext. apply hyp_rels_map_meta_rule_rels.
     Qed.
 
     Lemma all_rels_map_program p :
-      program.all_rels (map_program p) = map f (program.all_rels p).
+      program.all_rels (program.map_rel f p) = map f (program.all_rels p).
     Proof.
       cbv [program.all_rels]. rewrite concl_rels_map_program, hyp_rels_map_program.
       rewrite map_app. reflexivity.
@@ -1270,7 +1354,7 @@ Section RelMap.
 
     Lemma map_input_set_iff Q g1 g2 :
       (forall f1 f2, fact_equiv f1 f2 -> Q f1 <-> Q f2) ->
-      wf_fact map_rel g1 g2 ->
+      fact.wf map_rel g1 g2 ->
       Q g1 <-> (exists g, g2 = fact.map_rel f g /\ Q g).
     Proof.
       intros HQ Hg. apply wf_fact_map in Hg. subst. split; [eauto|].
@@ -1283,7 +1367,7 @@ Section RelMap.
       (forall f1 f2, fact_equiv f1 f2 -> Q f1 <-> Q f2) ->
       Forall (inj_on_elt map_rel) (program.concl_rels p) ->
       program.interp p Q fct <->
-        program.interp (map_program p)
+        program.interp (program.map_rel f p)
           (fun f' => exists g, f' = fact.map_rel f g /\ Q g) (fact.map_rel f fct).
     Proof.
       intros. apply (interp_wf_iff map_rel); auto using wf_program_map, map_input_set_iff.
@@ -1295,7 +1379,7 @@ Section RelMap.
       injective_on f (fact.rel fct :: program.all_rels p) ->
       (forall f1 f2, fact_equiv f1 f2 -> Q f1 <-> Q f2) ->
       program.interp p Q fct <->
-        program.interp (map_program p)
+        program.interp (program.map_rel f p)
           (fun f' => exists g, f' = fact.map_rel f g /\ Q g) (fact.map_rel f fct).
     Proof.
       intros. apply (interp_wf_iff_inj map_rel);
@@ -1309,83 +1393,83 @@ Section RelMap.
     Context {rel1 rel2 rel3 : Type}.
 
     Lemma wf_clause_flip (R : rel1 -> rel2 -> Prop) c1 c2 :
-      wf_clause R c1 c2 ->
-      wf_clause (fun y x => R x y) c2 c1.
-    Proof. cbv [wf_clause]. intuition. Qed.
+      clause.wf R c1 c2 ->
+      clause.wf (fun y x => R x y) c2 c1.
+    Proof. cbv [clause.wf]. intuition. Qed.
 
     Lemma wf_rule_flip (R : rel1 -> rel2 -> Prop) r1 r2 :
-      wf_rule R r1 r2 ->
-      wf_rule (fun y x => R x y) r2 r1.
+      rule.wf R r1 r2 ->
+      rule.wf (fun y x => R x y) r2 r1.
     Proof.
       destruct 1; constructor; try assumption;
         rewrite <- Forall2_flip_iff; eapply Forall2_impl; eauto using wf_clause_flip.
     Qed.
 
     Lemma wf_clause_pattern_flip (R : rel1 -> rel2 -> Prop) c1 c2 :
-      wf_clause_pattern R c1 c2 ->
-      wf_clause_pattern (fun y x => R x y) c2 c1.
-    Proof. cbv [wf_clause_pattern]. intuition. Qed.
+      clause_pattern.wf R c1 c2 ->
+      clause_pattern.wf (fun y x => R x y) c2 c1.
+    Proof. cbv [clause_pattern.wf]. intuition. Qed.
 
     Lemma wf_meta_rule_flip (R : rel1 -> rel2 -> Prop) mr1 mr2 :
-      wf_meta_rule R mr1 mr2 ->
-      wf_meta_rule (fun y x => R x y) mr2 mr1.
+      meta_rule.wf R mr1 mr2 ->
+      meta_rule.wf (fun y x => R x y) mr2 mr1.
     Proof.
-      cbv [wf_meta_rule]. intros. fwd.
+      cbv [meta_rule.wf]. intros. fwd.
       split; rewrite <- Forall2_flip_iff; eapply Forall2_impl; eauto using wf_clause_pattern_flip.
     Qed.
 
     Lemma wf_program_flip (R : rel1 -> rel2 -> Prop) p1 p2 :
-      wf_program R p1 p2 ->
-      wf_program (fun y x => R x y) p2 p1.
+      program.wf R p1 p2 ->
+      program.wf (fun y x => R x y) p2 p1.
     Proof.
-      cbv [wf_program]. intros. fwd.
+      cbv [program.wf]. intros. fwd.
       split; rewrite <- Forall2_flip_iff; eapply Forall2_impl;
         eauto using wf_rule_flip, wf_meta_rule_flip.
     Qed.
 
     Lemma wf_clause_comp (R : rel1 -> rel2 -> Prop) (S : rel2 -> rel3 -> Prop) c1 c2 c3 :
-      wf_clause R c1 c2 ->
-      wf_clause S c2 c3 ->
-      wf_clause (fun x z => exists y, R x y /\ S y z) c1 c3.
-    Proof. cbv [wf_clause]. intros. fwd. split; [eauto | congruence]. Qed.
+      clause.wf R c1 c2 ->
+      clause.wf S c2 c3 ->
+      clause.wf (fun x z => exists y, R x y /\ S y z) c1 c3.
+    Proof. cbv [clause.wf]. intros. fwd. split; [eauto | congruence]. Qed.
 
     Lemma wf_clauses_comp (R : rel1 -> rel2 -> Prop) (S : rel2 -> rel3 -> Prop) cs1 cs2 cs3 :
-      Forall2 (wf_clause R) cs1 cs2 ->
-      Forall2 (wf_clause S) cs2 cs3 ->
-      Forall2 (wf_clause (fun x z => exists y, R x y /\ S y z)) cs1 cs3.
+      Forall2 (clause.wf R) cs1 cs2 ->
+      Forall2 (clause.wf S) cs2 cs3 ->
+      Forall2 (clause.wf (fun x z => exists y, R x y /\ S y z)) cs1 cs3.
     Proof.
       intros. eapply Forall2_impl; [eapply Forall2_comp; eassumption|].
       intros ? ? Hab. cbv beta in Hab. fwd. eauto using wf_clause_comp.
     Qed.
 
     Lemma wf_rule_comp (R : rel1 -> rel2 -> Prop) (S : rel2 -> rel3 -> Prop) r1 r2 r3 :
-      wf_rule R r1 r2 ->
-      wf_rule S r2 r3 ->
-      wf_rule (fun x z => exists y, R x y /\ S y z) r1 r3.
+      rule.wf R r1 r2 ->
+      rule.wf S r2 r3 ->
+      rule.wf (fun x z => exists y, R x y /\ S y z) r1 r3.
     Proof. destruct 1; invert 1; constructor; eauto using wf_clauses_comp. Qed.
 
     Lemma wf_clause_pattern_comp (R : rel1 -> rel2 -> Prop) (S : rel2 -> rel3 -> Prop) c1 c2 c3 :
-      wf_clause_pattern R c1 c2 ->
-      wf_clause_pattern S c2 c3 ->
-      wf_clause_pattern (fun x z => exists y, R x y /\ S y z) c1 c3.
-    Proof. cbv [wf_clause_pattern]. intros. fwd. split; [eauto | congruence]. Qed.
+      clause_pattern.wf R c1 c2 ->
+      clause_pattern.wf S c2 c3 ->
+      clause_pattern.wf (fun x z => exists y, R x y /\ S y z) c1 c3.
+    Proof. cbv [clause_pattern.wf]. intros. fwd. split; [eauto | congruence]. Qed.
 
     Lemma wf_meta_rule_comp (R : rel1 -> rel2 -> Prop) (S : rel2 -> rel3 -> Prop) mr1 mr2 mr3 :
-      wf_meta_rule R mr1 mr2 ->
-      wf_meta_rule S mr2 mr3 ->
-      wf_meta_rule (fun x z => exists y, R x y /\ S y z) mr1 mr3.
+      meta_rule.wf R mr1 mr2 ->
+      meta_rule.wf S mr2 mr3 ->
+      meta_rule.wf (fun x z => exists y, R x y /\ S y z) mr1 mr3.
     Proof.
-      cbv [wf_meta_rule]. intros. fwd.
+      cbv [meta_rule.wf]. intros. fwd.
       split; (eapply Forall2_impl; [eapply Forall2_comp; eassumption|]);
         intros ? ? Hab; cbv beta in Hab; fwd; eauto using wf_clause_pattern_comp.
     Qed.
 
     Lemma wf_program_comp (R : rel1 -> rel2 -> Prop) (S : rel2 -> rel3 -> Prop) p1 p2 p3 :
-      wf_program R p1 p2 ->
-      wf_program S p2 p3 ->
-      wf_program (fun x z => exists y, R x y /\ S y z) p1 p3.
+      program.wf R p1 p2 ->
+      program.wf S p2 p3 ->
+      program.wf (fun x z => exists y, R x y /\ S y z) p1 p3.
     Proof.
-      cbv [wf_program]. intros. fwd.
+      cbv [program.wf]. intros. fwd.
       split; (eapply Forall2_impl; [eapply Forall2_comp; eassumption|]);
         intros ? ? Hab; cbv beta in Hab; fwd; eauto using wf_rule_comp, wf_meta_rule_comp.
     Qed.
